theories/Environment/GenEnv.v
@@ -1,0 +1,3 @@
+From Coq Require Import Classes.Morphisms.
+From Mecha Require Import Resource Typ Var.
+From DeBrLevel Require Import LevelInterface MapLevelInterface MapLevelD.
