theories/Syntax/Save.v
@@ -1,0 +1,152 @@
+From Coq Require Import Lia RelationClasses Classes.Morphisms.
+From Mecha Require Import Resource Term Typ RContext.
+From DeBrLevel Require Import LevelInterface.
+Import ResourceNotations TermNotations TypNotations RContextNotations.
+
+Module Save <: IsLvlET.
+
+Definition t : Type := ℜ * Λ * Τ * Τ.
+
+Definition eq (t t' : t) :=
+  let '(Rc,v,ty,ty1) := t in
+  let '(Rc',v',ty',ty1') := t' in 
+  (Rc = Rc')%rc /\ v = v' /\ ty = ty' /\ ty1 = ty1'.
+
+#[export] Instance eq_refl : Reflexive eq.
+Proof.
+  intros [[[Rc v] ty] ty1]; 
+  repeat split.
+Qed.
+
+#[export] Instance eq_sym : Symmetric eq.
+Proof.
+  intros [[[Rc v] ty] ty1] [[[Rc' v'] ty'] ty1'] [HeqRc [Heqv []]]; subst.
+  repeat split.
+  now symmetry.
+Qed.
+
+#[export] Instance eq_trans : Transitive eq.
+Proof.
+  intros [[[Rc v] ty] ty1] 
+         [[[Rc' v'] ty'] ty1'] 
+         [[[Rc'' v''] ty''] ty1'']
+         [HeqRc [Heqv []]] 
+         [HeqRc' [Heqv' []]]; subst.
+  repeat split.
+  now rewrite HeqRc.
+Qed. 
+
+#[export] Instance eq_equiv : Equivalence eq.
+Proof.
+  split.
+  - apply eq_refl.
+  - apply eq_sym.
+  - apply eq_trans.
+Qed.
+
+
+Definition shift (m n : resource) (tp : t) :=
+  let '(Rc,v,ty,ty') := tp in 
+  (([⧐ m – n] Rc)%rc,(Term.shift m n v)%tm,(Typ.shift m n ty)%ty,(Typ.shift m n ty')%ty).
+
+Definition Wf (m : resource) (tp : t) :=
+  let '(Rc,v,ty,ty') := tp in 
+  RContext.Wf m Rc /\ Term.Wf m v /\ Typ.Wf m ty /\ Typ.Wf m ty'.
+
+
+#[export] Hint Resolve eq_refl eq_sym eq_trans : core.
+
+Lemma eq_dec (t1 t2: t) : {eq t1 t2} + {~ eq t1 t2}.
+Proof. 
+  (* needs to define RContext as an OrderedMaps in order to get eq_dec lemma *)
+Admitted.
+
+(** **** [shift] properties *)
+
+Lemma shift_zero_refl (lb : lvl) (t : t) : eq (shift lb 0 t) t.
+Proof.
+  destruct t as [[[Rc v] ty] ty1]; simpl.
+  rewrite RContext.shift_zero_refl.
+  rewrite Term.shift_zero_refl.
+  do 2 rewrite Typ.shift_zero_refl.
+  repeat split.
+Qed.
+
+#[export] Instance shift_eq : 
+  Proper (Logic.eq ==> Logic.eq ==> eq ==> eq) shift.
+Proof. Admitted.
+
+Lemma shift_eq_iff (lb k : lvl) (t t1 : t) :
+  eq t t1 <-> eq (shift lb k t) (shift lb k t1).
+Proof.
+Admitted.
+
+Lemma shift_trans (lb k m : lvl) (t : t) :
+  eq (shift lb k (shift lb m t)) (shift lb (k + m) t).
+Proof.
+Admitted.
+
+Lemma shift_permute (lb k m : lvl) (t : t) :
+  eq (shift lb k (shift lb m t)) (shift lb m (shift lb k t)).
+Proof.
+Admitted.
+
+Lemma shift_permute_1 (lb k m : lvl) (t : t) :
+  eq (shift lb k (shift lb m t)) (shift (lb + k) m (shift lb k t)).
+Proof.
+Admitted.
+
+Lemma shift_permute_2 (lb k m n : lvl) (t : t) :
+  lb <= k -> eq (shift lb m (shift k n t)) (shift (k + m) n (shift lb m t)).
+Proof.
+Admitted.
+
+Lemma shift_unfold (lb k m : lvl) (t : t) :
+  eq (shift lb (k + m) t) (shift (lb + k) m (shift lb k t)). 
+Proof.
+Admitted.
+
+Lemma shift_unfold_1 (k m n : lvl) (t : t) :
+  k <= m -> m <= n -> 
+  eq (shift m (n - m) (shift k  (m - k) t)) (shift k (n - k) t).
+Proof.
+Admitted.
+
+(** **** [Wf] properties *)
+
+#[export] Instance Wf_iff : Proper (Logic.eq ==> eq ==> iff) Wf.
+Admitted.
+
+Lemma Wf_weakening (k m : lvl) (t : t) : (k <= m) -> Wf k t -> Wf m t.
+Proof.
+Admitted.
+
+Theorem shift_preserves_wf_1 (lb k m : lvl) (t : t) :
+  Wf k t -> Wf (k + m) (shift lb m t).
+Proof.
+Admitted.
+
+
+Theorem shift_preserves_wf (k m : lvl) (t : t) :
+  Wf k t -> Wf (k + m) (shift k m t).
+Proof. intros; now apply shift_preserves_wf_1. Qed. 
+
+Theorem shift_preserves_wf_zero (k : lvl) (t : t) :
+  Wf k t -> Wf k (shift k 0 t).
+Proof.
+Admitted.
+
+Lemma shift_preserves_wf_gen (lb k m n : lvl) (t : t) :
+    m <= n -> lb <= k -> m <= lb -> n <= k -> n - m = k - lb -> 
+    Wf lb t -> Wf k (shift m (n - m) t).
+Proof.
+Admitted.
+
+Lemma shift_preserves_wf_2 (m n : lvl) (t : t) :
+  m <= n -> Wf m t -> Wf n (shift m (n - m) t).
+Proof. 
+  intros Hle Hvt. 
+  eapply shift_preserves_wf_gen; eauto. 
+Qed.
+
+End Save.
